Factored out wk lemmas

LogicalRefinement/Typed.lean
@@ -4,144 +4,10 @@ import LogicalRefinement.Utils
 import LogicalRefinement.Tactics
 import LogicalRefinement.Typed.Context
 import LogicalRefinement.Typed.Basic
+import LogicalRefinement.Typed.Wk
 open Untyped
 open Annot
 open AnnotSort
-
-inductive WkCtx: Wk -> Context -> Context -> Type
-  | id: WkCtx Wk.id Γ Γ
-  | step {ρ Γ Δ H}: WkCtx ρ Γ Δ -> WkCtx ρ.step (H::Γ) Δ 
-  | lift {ρ Γ Δ k} {A: Untyped}: WkCtx ρ Γ Δ 
-    -> WkCtx ρ.lift ((Hyp.mk (A.wk ρ) k)::Γ) ((Hyp.mk A k)::Δ)
-
-def WkCtx.lift_loose: 
-  ρ' = ρ.lift -> A' = A.wk ρ -> WkCtx ρ Γ Δ -> WkCtx ρ' ((Hyp.mk A' k)::Γ) ((Hyp.mk A k)::Δ) := by {
-    intro Hρ HA R;
-    rw [Hρ, HA];
-    exact WkCtx.lift R
-  }
-
-def WkCtx.wk1 {Γ H}: WkCtx Wk.wk1 (H::Γ) Γ := WkCtx.step WkCtx.id
-
-theorem WkCtx.upgrade: WkCtx ρ Γ Δ 
-  -> WkCtx ρ Γ.upgrade Δ.upgrade := by {
-  intro R;
-  induction R with
-  | id => exact id
-  | step R => apply step; assumption
-  | lift R =>
-    simp only [Context.upgrade, Hyp.upgrade_wk_commute]
-    apply lift <;> assumption
-}
-
-theorem HasVar.wk:
-  (ρ: Wk) -> {Γ Δ: Context} -> (Hs: WkCtx ρ Γ Δ) ->
-  {n: Nat} -> {A: Untyped} -> {s: HypKind} ->
-  HasVar Δ A s n -> HasVar Γ (A.wk ρ) s (ρ.var n) 
-  := by {
-    intros ρ;
-    induction ρ <;> intro Γ Δ R <;> cases R;
-    case id => 
-      intros n A s H;
-      simp [H] 
-    case step ρ I Γ H R =>
-      intros n A s HΔ;
-      simp only [Untyped.step_wk1]
-      exact var_succ (I R HΔ)
-    case lift ρ I Γ Δ k A R =>
-      intros n A s HΔ;
-      cases HΔ with
-      | var0 =>
-        simp only [
-          Wk.lift,
-          Untyped.wk_composes,
-          Wk.var, Untyped.lift_wk1
-        ]
-        apply var0
-        assumption
-      | var_succ =>
-        simp only [
-          Wk.lift,
-          Untyped.wk_composes,
-          Wk.var, Nat.add, Untyped.lift_wk1
-        ]
-        apply var_succ
-        apply I
-        apply R
-        assumption
-  } 
-
-theorem HasType.wk {Δ a A} (HΔ: Δ ⊢ a: A):
-  {ρ: Wk} -> {Γ: Context} -> WkCtx ρ Γ Δ ->
-  (Γ ⊢ (a.wk ρ): (A.wk ρ)) := by {
-    induction HΔ;
-    case var I =>
-      intros
-      apply var
-      apply I
-      assumption
-      apply HasVar.wk
-      repeat assumption
-
-    all_goals (
-      intros ρ Γ R
-      simp only [
-        Untyped.wk, Annot.wk, term, proof, Untyped.subst0_wk,
-        Untyped.wk1
-      ] at *
-      constructor <;> 
-      rename_i' I5 I4 I3 I2 I1 I0 <;> 
-      (try rw [Untyped.alpha00_wk_comm (by simp)]) <;>
-      (try rw [Untyped.let_bin_ty_alpha_wk_pair]) <;>
-      (try rw [Untyped.let_bin_ty_alpha_wk_elem]) <;>
-      (try rw [Untyped.let_bin_ty_alpha_wk_repr]) <;>
-      (try rw [Untyped.let_bin_ty_alpha_wk_wit]) <;>
-      (first | apply I0 | apply I1 | apply I2 | apply I3 | apply I4 | apply I5) <;> 
-      simp only [<-Hyp.wk_components] <;> 
-      first 
-      | exact R
-      | (exact R.upgrade)
-      | {
-        repeat (apply WkCtx.lift_loose rfl; rfl)
-        exact R
-      }
-    )
-  }
-
---TODO: basic weakening helpers
-
-def HasType.wk1 {H} (Ha: Γ ⊢ a: A): (H::Γ) ⊢ a.wk1: A.wk1 
-:= wk Ha WkCtx.wk1
-
-def HasType.wk1_sort {H} (Ha: Γ ⊢ a: sort s): (H::Γ) ⊢ a.wk1: sort s 
-:= wk Ha WkCtx.wk1
-
--- def HasType.wk_val (Ha: HasType Γ a A) (HB: HasType Γ B (sort s))
---   : HasType ((Hyp.val B s)::Γ) a.wk1 A.wk1
---   := wk1_inner Ha HB HypKind.regular.val
-
--- def HasType.wk_gst (Ha: HasType Γ a A) (HB: HasType Γ B type)
---   : HasType ((Hyp.gst B)::Γ) a.wk1 A.wk1
---   := wk1_inner Ha HB HypKind.regular.gst
-
---TODO: basic examples
-
--- -- Simple examples
-
--- def HasType.arrow (HA: Γ ⊢ A: type) (HB: Γ ⊢ B: type)
---   : Γ ⊢ (arrow A B): type 
---   := pi HA (wk_sort HB HA)
-
--- def HasType.lam_id (HA: Γ ⊢ A: type)
---   : Γ ⊢ (Untyped.lam A (var 0)) ∈ Untyped.arrow A A
---   := lam HA (var0 HA)
-
--- def HasType.const_lam 
---   (HA: Γ ⊢ A: type) (HB: Γ ⊢ B: type) (Hb: Γ ⊢ b ∈ B)
---   : HasType Γ (Untyped.lam A b.wk1) (term (Untyped.arrow A B))
---   := lam HA (wk_expr Hb HA)
-
---TODO: substitution lemma
 
 --TODO: fill in with proper definition
 
@@ -214,8 +80,6 @@ theorem SubstCtx.upgrade (S: SubstCtx ρ Γ Δ): SubstCtx ρ Γ.upgrade Δ.upgra
   intro n A k H;
   sorry
 }
-
-theorem eta_helper {σ: Subst}: (λn => σ n) = σ := by simp
 
 theorem HasType.subst {Δ a A} (HΔ: Δ ⊢ a: A):
   {σ: Subst} -> {Γ: Context} -> SubstCtx σ Γ Δ ->
