LogicalRefinement/Typed/Wk.lean
@@ -1,0 +1,115 @@
+import LogicalRefinement.Untyped
+import LogicalRefinement.Untyped.Subst
+import LogicalRefinement.Utils
+import LogicalRefinement.Tactics
+import LogicalRefinement.Typed.Context
+import LogicalRefinement.Typed.Basic
+open Untyped
+open Annot
+open AnnotSort
+
+inductive WkCtx: Wk -> Context -> Context -> Type
+  | id: WkCtx Wk.id Γ Γ
+  | step {ρ Γ Δ H}: WkCtx ρ Γ Δ -> WkCtx ρ.step (H::Γ) Δ 
+  | lift {ρ Γ Δ k} {A: Untyped}: WkCtx ρ Γ Δ 
+    -> WkCtx ρ.lift ((Hyp.mk (A.wk ρ) k)::Γ) ((Hyp.mk A k)::Δ)
+
+def WkCtx.lift_loose: 
+  ρ' = ρ.lift -> A' = A.wk ρ -> WkCtx ρ Γ Δ -> WkCtx ρ' ((Hyp.mk A' k)::Γ) ((Hyp.mk A k)::Δ) := by {
+    intro Hρ HA R;
+    rw [Hρ, HA];
+    exact WkCtx.lift R
+  }
+
+def WkCtx.wk1 {Γ H}: WkCtx Wk.wk1 (H::Γ) Γ := WkCtx.step WkCtx.id
+
+theorem WkCtx.upgrade: WkCtx ρ Γ Δ 
+  -> WkCtx ρ Γ.upgrade Δ.upgrade := by {
+  intro R;
+  induction R with
+  | id => exact id
+  | step R => apply step; assumption
+  | lift R =>
+    simp only [Context.upgrade, Hyp.upgrade_wk_commute]
+    apply lift <;> assumption
+}
+
+theorem HasVar.wk:
+  (ρ: Wk) -> {Γ Δ: Context} -> (Hs: WkCtx ρ Γ Δ) ->
+  {n: Nat} -> {A: Untyped} -> {s: HypKind} ->
+  HasVar Δ A s n -> HasVar Γ (A.wk ρ) s (ρ.var n) 
+  := by {
+    intros ρ;
+    induction ρ <;> intro Γ Δ R <;> cases R;
+    case id => 
+      intros n A s H;
+      simp [H] 
+    case step ρ I Γ H R =>
+      intros n A s HΔ;
+      simp only [Untyped.step_wk1]
+      exact var_succ (I R HΔ)
+    case lift ρ I Γ Δ k A R =>
+      intros n A s HΔ;
+      cases HΔ with
+      | var0 =>
+        simp only [
+          Wk.lift,
+          Untyped.wk_composes,
+          Wk.var, Untyped.lift_wk1
+        ]
+        apply var0
+        assumption
+      | var_succ =>
+        simp only [
+          Wk.lift,
+          Untyped.wk_composes,
+          Wk.var, Nat.add, Untyped.lift_wk1
+        ]
+        apply var_succ
+        apply I
+        apply R
+        assumption
+  } 
+
+theorem HasType.wk {Δ a A} (HΔ: Δ ⊢ a: A):
+  {ρ: Wk} -> {Γ: Context} -> WkCtx ρ Γ Δ ->
+  (Γ ⊢ (a.wk ρ): (A.wk ρ)) := by {
+    induction HΔ;
+    case var I =>
+      intros
+      apply var
+      apply I
+      assumption
+      apply HasVar.wk
+      repeat assumption
+
+    all_goals (
+      intros ρ Γ R
+      simp only [
+        Untyped.wk, Annot.wk, term, proof, Untyped.subst0_wk,
+        Untyped.wk1
+      ] at *
+      constructor <;> 
+      rename_i' I5 I4 I3 I2 I1 I0 <;> 
+      (try rw [Untyped.alpha00_wk_comm (by simp)]) <;>
+      (try rw [Untyped.let_bin_ty_alpha_wk_pair]) <;>
+      (try rw [Untyped.let_bin_ty_alpha_wk_elem]) <;>
+      (try rw [Untyped.let_bin_ty_alpha_wk_repr]) <;>
+      (try rw [Untyped.let_bin_ty_alpha_wk_wit]) <;>
+      (first | apply I0 | apply I1 | apply I2 | apply I3 | apply I4 | apply I5) <;> 
+      simp only [<-Hyp.wk_components] <;> 
+      first 
+      | exact R
+      | (exact R.upgrade)
+      | {
+        repeat (apply WkCtx.lift_loose rfl; rfl)
+        exact R
+      }
+    )
+  }
+
+def HasType.wk1 {H} (Ha: Γ ⊢ a: A): (H::Γ) ⊢ a.wk1: A.wk1 
+:= wk Ha WkCtx.wk1
+
+def HasType.wk1_sort {H} (Ha: Γ ⊢ a: sort s): (H::Γ) ⊢ a.wk1: sort s 
+:= wk Ha WkCtx.wk1
